- Implement Queries that return multilists. - List Implementations of queries that return multisets. - Still have to modify insertion to not return duplicates.

src/QueryStructure/QuerySpecs/QueryQSSpecs.v
@@ -1,4 +1,4 @@
-Require Import List String Ensembles
+Require Import List String Ensembles Sorting.Permutation
         Computation.Core
         ADT.ADTSig ADT.Core
         ADTNotation.StringBound ADTNotation.BuildADT ADTNotation.BuildADTSig
@@ -11,49 +11,51 @@ Require Import List String Ensembles
 
 Open Scope comp.
 
-Definition QueryResultEquiv
+Definition Query_For {ResultT}
+           (bod : Comp (list ResultT)) : Comp (list ResultT) :=
+  result <- bod;
+  {l | Permutation result l}.
+
+Notation "'For' bod" := (Query_For bod) : QuerySpec_scope.
+
+Definition flatten_CompList {A} (c : list (Comp (list A))) :=
+  fold_right (fun (b : Comp (list A)) (a : Comp (list A)) =>
+                l <- b;
+              l' <- a;
+              ret (l ++ l')) (ret []) c.
+
+Definition QueryResultComp
            {QueryT ResultT}
            (queriedEnsemble : Ensemble QueryT)
-           (resultEnsemble : QueryT -> Ensemble (list ResultT))
-           (resultList : list ResultT)
+           (resultEnsemble : QueryT -> Comp (list ResultT))
   :=
     (* First construct a list that contains each element in the query list
        (expressed as an ensemble) paired with its result list.
        Then flatten the result and compare with [resultList].*)
-    exists queriedList : list (QueryT * (list ResultT)),
-       (forall el : QueryT * (list ResultT),
-          List.In el queriedList <->
-          (In _ queriedEnsemble (fst el) /\ In _ (resultEnsemble (fst el)) (snd el)))
-       /\ resultList = flatten (map snd queriedList).
+    queriedList <- {queriedList | EnsembleListEquivalence queriedEnsemble queriedList };
+    flatten_CompList (map resultEnsemble queriedList).
 
 Definition Query_In (qs : QueryStructureHint) {ResultT} (R : _)
            (bod : @Tuple (schemaHeading
                             (QSGetNRelSchema qsSchemaHint' R))
-                  -> Ensemble (list ResultT))
-           (results : list ResultT) :=
-  QueryResultEquiv (GetUnConstrRelation (DropQSConstraints qsHint) R) bod results.
+                  -> Comp (list ResultT)) :=
+  QueryResultComp (GetUnConstrRelation (DropQSConstraints qsHint) R) bod.
 
 Notation "( x 'in' R ) bod" :=
   (Query_In _ {| bindex := R%string |} (fun x => bod)) : QuerySpec_scope.
 
-(* [Query_Return] terminates the trace with a unit value. *)
-Definition Query_Return {A : Type} (a : A) (el : list A) := (el = [a]).
+(* [Query_Return] returns the singleton list. *)
+Definition Query_Return {ResultT : Type} (a : ResultT) := ret [a].
 
 Notation "'Return' t" :=
   (Query_Return t%Tuple) : QuerySpec_scope.
 
 Definition Query_Where
-           {A : Type} (P : Prop) (bod : Ensemble (list A)) (a : list A) :=
-  P /\ bod a.
+           {ResultT : Type} (P : Prop) (bod : Comp (list ResultT)) :=
+  {l | P -> bod ↝ l /\ ~ P -> l = []}.
 
 Notation "'Where' p bod" :=
   (Query_Where p%Tuple bod) : QuerySpec_scope.
-
-Definition Query_For {ResultT}
-           (bod : Ensemble (list ResultT)) : Comp (list ResultT) :=
-  {l | bod l}.
-
-Notation "'For' bod" := (Query_For bod) : QuerySpec_scope.
 
 (* The spec for a count of the number of tuples in a relation. *)
 Definition Count {A} (rows : Comp (list A)) : Comp nat :=
