examples/Trivial.v
@@ -22,22 +22,6 @@ Definition MySig : ADTSig :=
     "YoungOwners'Breeds" : rep × nat → rep × list string
   }.
 
-Definition MySpec : ADT MySig :=
-  QueryADTRep MySchema {
-    const "Empty" (_ : unit) : rep := empty,
-
-    query "YoungOwners'Breeds" ( ageLimit : nat ) : list string :=
-      For (d in "Dog") (o in "Person")
-      Where (o!"Age" > ageLimit)
-      Where (d!"Owner" = o!"Name")
-      Return d!"Breed"
-}.
-
-Definition MyListImpl_abs
-           (or : UnConstrQueryStructure MySchema)
-           (nr : list Person * list Dog) : Prop :=
-  or!"Person" ≃ fst nr /\ or!"Dog" ≃ snd nr.
-
 Definition People := GetRelationKey MySchema "Person".
 Definition Dogs := GetRelationKey MySchema "Dog".
 
@@ -47,6 +31,25 @@ Definition Name := GetAttributeKey People "Name".
 Definition Owner := GetAttributeKey Dogs "Owner".
 Definition Breed := GetAttributeKey Dogs "Breed".
 
+
+Definition MySpec : ADT MySig :=
+  QueryADTRep MySchema {
+    const "Empty" (_ : unit) : rep := empty,
+
+    query "YoungOwners'Breeds" ( ageLimit : nat ) : list string :=
+      For (d in "Dog") (o in "Person")
+      Where (o Age > ageLimit)
+      Where (d Owner = o Name)
+      Return (d Breed)
+}.
+
+Definition MyListImpl_abs
+           (or : UnConstrQueryStructure MySchema)
+           (nr : list Person * list Dog) : Prop :=
+  or!"Person" ≃ fst nr /\ or!"Dog" ≃ snd nr.
+
+Opaque Query_For.
+
 Definition My :
   Sharpened MySpec.
 Proof.
@@ -54,90 +57,31 @@ Proof.
 
   start honing QueryStructure.
 
-  (* Need to fix TypeClass lookup for this to go through. *)
-  (* hone method "YoungOwners'Breeds".
-
-
-  etransitivity.
-  setoid_rewrite refine_For_Equivalent_Trace_Ensembles;
-    [ reflexivity
-    | eapply (Equivalent_Swap_In r_n (GetRelationKey MySchema "Dog")
-                                 (GetRelationKey MySchema "Person")
-                                 (fun (d : Dog) (o : Person) =>
-                                    Where (o!"Age" > n)
-                                          Where (d!"Owner" = o!"Name")
-                                          Return d!"Breed"))].
-  etransitivity.
-  setoid_rewrite refine_For_Equivalent_Trace_Ensembles.
-  reflexivity.
-  eapply Equivalent_Under_In; simpl.
-  intros; generalize (Equivalent_Swap_In_Where r_n {|bindex := "Dog" |}
-          (fun (tup : Person) (tup' : Dog) =>
-             Where (tup!"Owner" = tup!"Name")
-                   Return tup'!"Breed")).
-                      ).
-  rewrite refine_Query_For_In_Equivalent;
-    [ | apply Equivalent_Swap_In_Where with (qs := _)]; cbv beta.
-  finish honing. *)
-
   hone representation using MyListImpl_abs.
   implement_empty_list "Empty" MyListImpl_abs.
 
   hone method "YoungOwners'Breeds".
   {
+    simpl.
     unfold MyListImpl_abs in H; split_and.
     setoid_rewrite refineEquiv_pick_ex_computes_to_and.
     simplify with monad laws.
-    simpl.
-    etransitivity.
-    { setoid_rewrite refine_For_Equivalent_Trace_Ensembles;
-      [ reflexivity | ].
-      eapply (@Equivalent_UnConstr_In_EnsembleListEquivalence 
-                _ _ _ c _
-                (snd r_n)
-                (fun b : Tuple =>
-                   UnConstrQuery_In c People
-                                    (fun o : Person =>
-                                       Where (o Age > n)
-                                             Where (b Owner = o Name)
-                                             Return (b Breed) ))).
-      eauto.
-    }
-    simpl; etransitivity.
-    { apply refine_bind.
-      eapply refine_For_Equivalent_Trace_Ensembles.
-      eapply (@Equivalent_Join_Lists string unit _ _ c People (snd r_n)
-                                 _ (fun el (o : Person) =>
-         Where (o Age > n)
-               Where (el Owner = o Name)
-               Return (el Breed)) H1).
-      unfold pointwise_relation; intros.
-      higher_order_1_reflexivity.
-    } simpl; etransitivity.
-    { apply refine_bind.
-      eapply refine_For_Equivalent_Trace_Ensembles.
-      eapply Equivalent_List_In_Where with (P_dec := _).
-  simpl; intros.
-  eapply X.
-  setoid_rewrite Equivalent_Join_Lists; [ | eassumption ].
-  simpl in X.
-  eapply X.
-  setoid_rewrite Equivalent_UnConstr_In_EnsembleListEquivalence.
-    [ | eassumption ].
-  setoid_rewrite Equivalent_List_In_Where with (P_dec := _).
-  setoid_rewrite Equivalent_Join_Lists; [ | eassumption ].
-  setoid_rewrite Equivalent_List_In_Where with (P_dec := _).
-  setoid_rewrite refine_For_List_Return.
-  simplify with monad laws.
-  unfold MyListImpl_abs.
-  setoid_rewrite refineEquiv_pick_pair_pair.
-  setoid_rewrite refineEquiv_pick_eq'.
-  simplify with monad laws.
-  rewrite refine_pick_val by eassumption.
-  simplify with monad laws.
-  rewrite refine_pick_val by eassumption.
-  simplify with monad laws.
-  finish honing.
+    rewrite refine_List_Query_In; eauto.
+    rewrite refine_Join_List_Query_In; eauto.
+    rewrite refine_List_Query_In_Where.
+    rewrite refine_List_Query_In_Where.
+    rewrite refine_List_For_Query_In_Return;
+      simplify with monad laws; simpl.
 
+    setoid_rewrite refineEquiv_pick_pair_pair.
+    setoid_rewrite refineEquiv_pick_eq'.
+    simplify with monad laws.
+    rewrite refine_pick_val by eassumption.
+    simplify with monad laws.
+    rewrite refine_pick_val by eassumption.
+    simplify with monad laws.
+    finish honing.
+  }
+  
   finish sharpening.
 Defined.
